src/SemFacts.v
@@ -1,0 +1,227 @@
+Require Import String List Program.Equality.
+Require Import Lib.CommonTactics Lib.FMap Lib.Struct.
+Require Import Syntax Semantics.
+
+Set Implicit Arguments.
+
+Theorem staticDynCallsRules m o name a u cs r:
+  In (name :: a)%struct (getRules m) ->
+  SemAction o (a type) u cs r ->
+  forall f, M.In f cs -> In f (getCalls m).
+Proof.
+  admit.
+Qed.
+
+Theorem staticDynCallsMeths m o name a u cs r:
+  In (name :: a)%struct (getDefsBodies m) ->
+  forall argument,
+    SemAction o (projT2 a type argument) u cs r ->
+    forall f, M.In f cs -> In f (getCalls m).
+Proof.
+  admit.
+Qed.
+
+Theorem staticDynCallsSubstep m o u rm cs:
+  Substep m o u rm cs ->
+  forall f, M.In f cs -> In f (getCalls m).
+Proof.
+  intro H.
+  dependent induction H; simpl in *; intros.
+  - apply (M.F.P.F.empty_in_iff) in H; intuition.
+  - apply (M.F.P.F.empty_in_iff) in H; intuition.
+  - eapply staticDynCallsRules; eauto.
+  - destruct f as [name a]; simpl in *.
+    eapply staticDynCallsMeths; eauto.
+Qed.
+
+Theorem staticDynDefsSubstep m o u far cs:
+  Substep m o u (Meth (Some far)) cs ->
+  List.In (attrName far) (getDefs m).
+Proof.
+  intros.
+  dependent induction H; simpl in *.
+  unfold getDefs in *.
+  clear - HIn.
+  induction (getDefsBodies m).
+  - intuition.
+  - simpl in *.
+    destruct HIn.
+    + subst.
+      left; intuition.
+    + right; intuition.
+Qed.
+
+Theorem staticDynCallsSubsteps m o ss:
+  forall f, M.In f (calls (foldSSLabel (m := m) (o := o) ss)) -> In f (getCalls m).
+Proof.
+  intros.
+  induction ss; simpl in *.
+  - exfalso.
+    apply (proj1 (M.F.P.F.empty_in_iff _ _) H).
+  - unfold addLabelLeft, mergeLabel in *.
+    destruct a.
+    simpl in *.
+    destruct unitAnnot.
+    + destruct (foldSSLabel ss); simpl in *.
+      pose proof (M.union_In H) as sth.
+      destruct sth.
+      * apply (staticDynCallsSubstep substep); intuition.
+      * intuition.
+    + destruct (foldSSLabel ss); simpl in *.
+      dependent destruction o0; simpl in *.
+      * dependent destruction a; simpl in *.
+        pose proof (M.union_In H) as sth.
+        { destruct sth.
+          - apply (staticDynCallsSubstep substep); intuition.
+          - intuition.
+        }
+      * pose proof (M.union_In H) as sth.
+        { destruct sth.
+          - apply (staticDynCallsSubstep substep); intuition.
+          - intuition.
+        }
+Qed.
+
+Theorem staticDynDefsSubsteps m o ss:
+  forall f, M.In f (defs (foldSSLabel (m := m) (o := o) ss)) -> In f (getDefs m).
+Proof.
+  intros.
+  induction ss; simpl in *.
+  - exfalso.
+    apply (proj1 (M.F.P.F.empty_in_iff _ _) H).
+  - unfold addLabelLeft, mergeLabel in *.
+    destruct a.
+    simpl in *.
+    destruct unitAnnot.
+    + destruct (foldSSLabel ss); simpl in *.
+      rewrite M.union_empty_L in H.
+      intuition.
+    + destruct (foldSSLabel ss); simpl in *.
+      dependent destruction o0; simpl in *.
+      * dependent destruction a; simpl in *.
+        pose proof (M.union_In H) as sth.
+        { destruct sth.
+          - apply M.F.P.F.add_in_iff in H0.
+            destruct H0.
+            + subst.
+              apply (staticDynDefsSubstep substep).
+            + exfalso; apply ((proj1 (M.F.P.F.empty_in_iff _ _)) H0).
+          - intuition.
+        }
+      * rewrite M.union_empty_L in H.
+        intuition.
+Qed.
+
+Lemma hide_mergeLabel:
+  forall l1 l2,
+    M.Disj (defs l1) (defs l2) ->
+    M.Disj (calls l1) (calls l2) ->
+    hide (mergeLabel l1 l2) = mergeLabel (hide l1) (hide l2).
+Proof.
+  destruct l1 as [ann1 ds1 cs1], l2 as [ann2 ds2 cs2].
+  unfold hide, mergeLabel; simpl; f_equal; admit.
+Qed.
+
+Lemma substep_rule_dms_weakening:
+  forall regs rules dms1 or u r cs,
+    Substep (Mod regs rules dms1) or u (Rle r) cs ->
+    forall dms2,
+      Substep (Mod regs rules dms2) or u (Rle r) cs.
+Proof.
+  intros; inv H.
+  - constructor; auto.
+  - eapply SingleRule; eauto.
+Qed.
+
+Lemma substep_meth_none_dms_weakening:
+  forall regs rules dms1 or u cs,
+    Substep (Mod regs rules dms1) or u (Meth None) cs ->
+    forall dms2,
+      Substep (Mod regs rules dms2) or u (Meth None) cs.
+Proof. intros; inv H; constructor; auto. Qed.
+
+Lemma substepsInd_dms_weakening:
+  forall regs rules dms or u l,
+    SubstepsInd (Mod regs rules dms) or u l ->
+    forall filt,
+      M.KeysDisj (defs (hide l)) filt ->
+      SubstepsInd (Mod regs rules (filterDms dms filt)) or u (hide l).
+Proof.
+  induction 1; intros; [constructor|subst].
+  destruct sul as [sr|[[sdmn sdmv]|]].
+
+  - eapply SubstepsCons.
+    Focus 5.
+    + rewrite hide_mergeLabel.
+      * f_equal.
+        instantiate (1:= scs); instantiate (1:= Rle sr).
+        unfold hide, getLabel; simpl; f_equal.
+        apply M.subtractKV_empty_2.
+      * simpl; apply M.Disj_empty_1.
+      * inv H1; dest; simpl; auto.
+    + apply IHSubstepsInd.
+      admit.
+    + eapply substep_rule_dms_weakening; eauto.
+    + admit.
+    + auto.
+
+  - admit.
+    
+  - eapply SubstepsCons.
+    Focus 5.
+    + rewrite hide_mergeLabel.
+      * f_equal.
+        instantiate (1:= scs); instantiate (1:= Meth None).
+        unfold hide, getLabel; simpl; f_equal.
+        apply M.subtractKV_empty_2.
+      * simpl; apply M.Disj_empty_1.
+      * inv H1; dest; simpl; auto.
+    + apply IHSubstepsInd.
+      admit.
+    + eapply substep_meth_none_dms_weakening; eauto.
+    + admit.
+    + auto.
+Qed.
+
+Lemma hide_idempotent:
+  forall (l: LabelT), hide l = hide (hide l).
+Proof.
+  intros; destruct l as [ann ds cs].
+  unfold hide; simpl; f_equal;
+  apply M.subtractKV_idempotent.
+Qed.
+
+Lemma stepInd_dms_weakening:
+  forall regs rules dms or nr l,
+    StepInd (Mod regs rules dms) or nr l ->
+    forall filt,
+      M.KeysDisj (defs l) filt ->
+      StepInd (Mod regs rules (filterDms dms filt)) or nr l.
+Proof.
+  induction 1; intros.
+  rewrite hide_idempotent.
+  constructor.
+  - apply substepsInd_dms_weakening; auto.
+  - rewrite <-hide_idempotent.
+    admit.
+Qed.
+
+Lemma step_dms_weakening:
+  forall regs rules dms or nr l,
+    Step (Mod regs rules dms) or nr l ->
+    forall filt,
+      M.KeysDisj (defs l) filt ->
+      Step (Mod regs rules (filterDms dms filt)) or nr l.
+Proof.
+  intros; apply step_consistent; apply step_consistent in H.
+  apply stepInd_dms_weakening; auto.
+Qed.
+
+Lemma merge_preserves_step:
+  forall m or nr l,
+    Step m or nr l ->
+    Step (Mod (getRegInits m) (getRules m) (getDefsBodies m)) or nr l.
+Proof.
+  admit.
+Qed.
+
